ProbabilismWP.fst
@@ -1,0 +1,381 @@
+module ProbabilismWP
+
+(* Approach with post -> real WP and with supremum axiom *)
+
+open FStar.Real
+open FStar.Tactics
+open FStar.Tactics.Builtins
+open FStar.IndefiniteDescription
+open FStar.FunctionalExtensionality
+
+let pr = r:real{r >=. zero}
+let prob_post (a:Type) = a -> Tot pr
+// TODO: add monotonicity
+let prob_wp (a:Type) = prob_post a ^-> pr
+
+assume type distribution (a:Type) : Type
+
+assume val point_distribution (#a:Type) (x:a) : distribution a
+
+assume val uniform_distribution (#a:Type) (x:list a{Cons? x}) : distribution a
+
+let prob_wp_eqI #a (wp1 wp2: prob_wp a) :
+    Lemma (requires (forall post. wp1 post = wp2 post))
+          (ensures (wp1 == wp2)) =
+    assert (feq wp1 wp2);
+    assert (wp1 == wp2)
+
+let prob a (w:prob_wp a): Tot Type0 =
+  distribution a // TODO: require w to hold
+
+let prob_wreturn #a x : prob_wp a =
+  on _ (fun post -> post x)
+
+let prob_return a (x:a) : prob a (prob_wreturn x) = 
+  point_distribution x
+
+let prob_wbind #a #b (w1:prob_wp a) (w2:a -> prob_wp b) : prob_wp b = 
+  on _ (fun post -> w1 (fun x -> w2 x post))
+
+let prob_wbind_beta #a #b (w1:prob_wp a) (w2:a -> prob_wp b) (post:prob_post b) :
+  Lemma (prob_wbind w1 w2 post == w1 (fun x -> w2 x post)) = ()
+
+let prob_bind a b (w1:prob_wp a) (w2:a -> prob_wp b)
+      (f: prob a w1) (g: (x:a -> prob b (w2 x))) : prob b (prob_wbind w1 w2) =
+   admit()   
+
+// w1 is a more restrictive wp than w2
+let stronger #a (w1 w2:prob_wp a) = forall post. w1 post >=. w2 post
+
+let strongerI #a (w1 w2:prob_wp a) :
+  Lemma (requires forall post. w1 post >=. w2 post)
+        (ensures w1 `stronger` w2) = ()
+
+let prob_wp_stronger_eq #a (w1 w2:prob_wp a) :
+    Lemma (requires w1 `stronger` w2 /\ w2 `stronger` w1)
+    	  (ensures w1 == w2) = 
+    assert (w1 == w2) by (apply_lemma (`prob_wp_eqI))
+
+let prob_subcomp a (w1 w2 : prob_wp a) (f:prob a w1) : 
+                 Pure (prob a w2) (requires w1 `stronger` w2) (ensures (fun _ -> True)) =
+  f
+
+let ite_prob a (#w1 #w2 : prob_wp a) (f: prob a w1) (g: prob a w2) (b: bool) : Type =
+  prob a (if b then w1 else w2)
+
+total
+reflectable
+layered_effect { PROB : (a:Type) -> (wp:prob_wp a) -> Effect with 
+  repr = prob;
+  return = prob_return; 
+  bind = prob_bind;
+  subcomp = prob_subcomp;
+  if_then_else = ite_prob
+  }
+
+assume val real_numbers_complete: unit -> Lemma(
+  forall (p: real->bool) low high.
+  p low ==> not (p high) ==> (forall x y. x >=. y ==> p x ==> p y) ==>
+  (exists sup. (forall x. x <. sup ==> p x) /\ (forall x. x >. sup ==> not (p x))))
+
+// TODO: add requires, ensures, define
+assume val largest (p: pr -> Type0) : pr
+
+let lift_pure_prob_wp #a (wp:pure_wp a) : prob_wp a =
+    on _ (fun (post:prob_post a) -> largest (fun (p:pr) -> wp (fun x -> p <=. post x)))
+
+let lift_pure_prob a (wp:pure_wp a) (f: eqtype_as_type unit -> PURE a wp) : 
+   prob a (lift_pure_prob_wp wp) =
+   assume False; // TODO
+   point_distribution (f ())
+
+sub_effect PURE ~> PROB = lift_pure_prob
+
+effect Prob a (wp: prob_post a -> pr) = PROB a (on _ wp)
+effect ProbAny (a:Type) = Prob a (fun post -> 0.0R)
+
+let coin () : Prob bool (fun (post) -> (post true +. post false) /. two) =
+  PROB?.reflect (uniform_distribution [true;false])
+
+let test1 () : Prob bool (fun post -> (post true +. post false) /. two) = coin ()
+
+let test2 () : ProbAny bool = coin ()
+
+let test3 x : Prob string (prob_wreturn x) 
+by (admit_all()) = assume False; x
+
+let test4 () : PROB string (prob_wreturn "hello") = test3 "hello"
+
+let f (b:bool) : nat = if b then 0 else 1
+
+irreducible
+let bind_return #a #b (wp1:prob_wp a) (f:a->b) : Lemma(prob_wbind wp1 (fun x -> prob_wreturn (f x))
+                                  == on _ (fun(post:prob_post b) -> wp1 (fun x -> post (f x))))
+  [SMTPat (prob_wbind wp1 (fun x -> prob_wreturn (f x)))]                                 
+        =
+  admit()				     
+
+irreducible
+let return_bind #a #b (x:a) (wp2:a -> prob_wp b) : Lemma(prob_wbind (prob_wreturn x) wp2 == wp2 x) 
+  [SMTPat (prob_wbind (prob_wreturn x) wp2)]
+  =
+  admit()
+
+let test5 () : Prob nat (fun post -> (post 0 +. post 1) /. two) =
+  let c : bool = coin() in
+  f c
+
+let prob_wbind_on #a #b (wp1:prob_wp a) (wp2:a -> prob_wp b) : 
+  Lemma(prob_wbind (on (prob_post a) #pr wp1) wp2 == prob_wbind wp1 wp2)
+  [SMTPat (prob_wbind (on _ wp1) wp2)]
+  = ()
+
+(*
+open FStar.Tactics.Simplifier
+
+let equals_cong #t a b a' b' : Lemma
+  (requires a == a' /\ b == b')
+  (ensures (a == b) <==> (a' == b')) = ()
+
+let conversion (relation:term) = term -> Tac (term * (unit -> Tac unit))
+
+let dump_conversion (#relation:term) (msg:string) (c:conversion relation) : conversion relation = (fun t ->
+  print (msg ^ " " ^ term_to_string t); 
+  c t)
+
+let equals = (`(==))
+
+val id_conversion : conversion equals
+let id_conversion t =
+  (t, (fun () -> fail "id_conversion"))
+
+let iff = (`(<==>))
+
+val iff_id_conversion : conversion iff
+let iff_id_conversion t =
+  (t, (fun () -> fail "iff_id_conversion"))
+
+let cut_conversion #relation (c:conversion relation) (t:term) : Tac binder =
+  let (t', tac) = c t in
+  let thm = (`(`#relation) (`#t) (`#t')) in
+  
+
+let xxx (a:nat) : nat by (
+//  let (res, tac) = (dump_conversion "test" iff_id_conversion) (`(forall a. a)) in
+  let h = cut_conversion iff_id_conversion (`(forall a. a)) in
+  dump ""
+) = a+a
+*)
+
+(* assert (prob_wbind (on_domain (prob_post bool)
+              (fun (post) -> (post true +. post false) /. two))
+          (fun (x) -> prob_wreturn 0)
+          ==
+          prob_wbind (on_domain (prob_post bool)
+              (fun (post:prob_post bool) -> (post true +. post false) /. two))
+          (fun (x:bool) -> prob_wreturn 0)
+          )
+
+*)
+
+
+(* let x =
+assert (forall a b (x y:a). a `subtype_of` b ==> eq2 #a x y ==> eq2 #b x y) *)
+
+let test6 () : Prob nat (fun p -> p 0)
+=
+  let c : bool = coin() in 0
+
+let on_beta #a #b (f:_->_) x : Lemma(on a #b f x == f x) = ()
+
+(*let wrong #a (w1 w2: prob_wp a) : Lemma(w1 `stronger` w2) 
+[SMTPat (w1 `stronger` w2) ]
+= admit() *)
+
+let bool_simp1 () : Lemma((true = true) == true) = ()
+let bool_simp2 () : Lemma((false = true) == false) = ()
+let bool_simp3 () : Lemma(~true == False) = ()
+let bool_simp4 () : Lemma(~false == True) = ()
+
+
+assume val ifte : #(a:Type) -> (c:Type0) -> (t:a) -> (e:a) -> a
+
+let largest_single c f : 
+Lemma(largest (fun (p:pr) -> c ==> f p) == ifte c (largest f) 1.0R)
+[SMTPat (largest (fun (p:pr) -> c ==> f p))]
+= assume False
+
+let simp1 #a k f :
+Lemma((forall k. (forall (x:a). f x ==> k x) ==> (forall (x:a). k x))
+==
+(forall (x:a). f x))
+[SMTPat (forall k. (forall (x:a). f x ==> k x) ==> (forall (x:a). k x))]
+= assume False
+
+let probr #a (x:a) : Prob a (prob_wreturn x) by (admit_all()) = x
+
+let simp2 #a c f :
+  Lemma((forall (x:a). c == x ==> f x) == f c) = assume False
+
+let simplify_pure_null_wp_ax1 #a : Lemma(pure_null_wp a (fun _ -> True) == True) = ()
+
+let simplify_b2t_true () : Lemma(b2t true == True) = ()
+let simplify_True_and p : Lemma((True /\ p) == auto_squash p) = ()
+let simplify_and_True p : Lemma((p /\ True) == auto_squash p) = ()
+let simplify_auto_squash_auto_squash p : Lemma(auto_squash (auto_squash p) == auto_squash p) = ()
+
+let simplify_auto_squash_implies p q : Lemma((auto_squash p ==> q) == (p ==> q)) = ()
+let simplify_implies_auto_squash p q : Lemma((p ==> auto_squash q) == (p ==> q)) = ()
+
+let simplfify_eq_true b : Lemma((b = true) == b) = ()
+
+let simplify_lift_pure_prob_wp_auto_squash f : Lemma(lift_pure_prob_wp (fun post -> auto_squash (f post)) == lift_pure_prob_wp (fun post -> f post)) = admit()
+
+//let simplify_lift_pure_prob_wp_trivial (#a:Type) (x:a) : Lemma(lift_pure_prob_wp (fun (post:pure_post a) -> (post x)) == (fun (post:prob_post a) -> post x)) = admit()
+
+let simplify_lift_pure_prob_wp_pure_return (#a:Type) (x:a) : Lemma(lift_pure_prob_wp (pure_return a x) == prob_wreturn x) = admit()
+
+let simplify_pure_return (#a: Type) (x: a) :
+  Lemma((fun post -> post x) == pure_return a x) = admit()
+
+let simplify_pure_return' (#a: Type) (x: a) :
+  Lemma((fun post -> auto_squash (post x)) == pure_return a x) = admit()
+
+let pure_admit_wp (a:Type) : pure_wp a = (fun (p: pure_post a) -> True)
+
+let simplify_cond_pure_return (#a: Type) (c: Type) (x: a) :
+  Lemma((fun post -> c ==> post x) == ifte c (pure_return a x) (pure_admit_wp a)) = admit()
+
+//let simplify_pure_return'' () : Lemma((fun post -> auto_squash (post ())) == pure_return unit ()) = simplify_pure_return' ()
+
+let ifte_lift (#a:Type) (#b:Type) (f:a->b) (c:Type) (x y: a) : Lemma(f (ifte c x y) == ifte c (f x) (f y)) = admit()
+
+
+assume val prob_admit_wp : (a:Type) -> prob_wp a (* infinity *)
+
+let ifte_lift_lift_pure_prob_wp (#a:Type) (c:Type) (x y: pure_wp a) :
+  Lemma(lift_pure_prob_wp (ifte c x y) == ifte c (lift_pure_prob_wp x) (lift_pure_prob_wp y)) 
+  = ifte_lift lift_pure_prob_wp c x y
+
+
+let ifte_lift_prob_wbind (#a:Type) (#b:Type) (c:Type) (x y: prob_wp a) (wp2:a->prob_wp b):
+  Lemma(prob_wbind (ifte c x y) wp2 == ifte c (prob_wbind x wp2) (prob_wbind y wp2)) 
+  = admit()
+
+(*let tmp c = ifte_lift_prob_wbind c
+  (lift_pure_prob_wp (pure_return unit ())) (prob_admit_wp unit)
+                  (fun _ x -> prob_wreturn 0 x)*)
+
+let simplify_if (#a:Type) (c:bool) (t e: bool->a) :
+  Lemma((if c then t c else e c) == (if c then t true else e false)) = ()
+
+let lift_pure_prob_wp_pure_admit_wp a : 
+  Lemma(lift_pure_prob_wp (pure_admit_wp a) == prob_admit_wp a) = admit()
+
+let prob_wbind_prob_admit (#a:Type) (#b:Type) (wp2:a->prob_wp b) :
+  Lemma(prob_wbind (prob_admit_wp a) wp2 == prob_admit_wp b) = admit()
+
+let rec simplifier () : Tac unit =
+  l_to_r [`simplify_if];
+  l_to_r [`simplify_pure_null_wp_ax1];
+  l_to_r [`simplify_lift_pure_prob_wp_pure_return];
+  l_to_r [`simplfify_eq_true];
+  l_to_r [`simplify_pure_return];
+  l_to_r [`simplify_pure_return'];
+  l_to_r [`simplify_cond_pure_return];
+  l_to_r [`ifte_lift_lift_pure_prob_wp];
+//  l_to_r [`lift_pure_prob_wp_pure_admit_wp];
+  l_to_r [`ifte_lift_prob_wbind];
+//  l_to_r [`prob_wbind_prob_admit];
+//  l_to_r [`bind_return];
+
+  ()
+//  if goal = cur_goal() then ()
+//  else simplifier()
+//
+let test8a c : Prob nat 
+//(prob_wreturn (if c then 0 else 1))
+(fun post -> 0.0R)
+by (
+dump"before";
+simpl ();
+  l_to_r [`simplify_if];
+  l_to_r [`simplify_pure_null_wp_ax1];
+  l_to_r [`simplify_lift_pure_prob_wp_pure_return];
+  l_to_r [`simplfify_eq_true];
+  l_to_r [`simplify_pure_return];
+  l_to_r [`simplify_pure_return'];
+  l_to_r [`simplify_cond_pure_return];
+  l_to_r [`ifte_lift_lift_pure_prob_wp];
+  l_to_r [`lift_pure_prob_wp_pure_admit_wp];
+//simplifier ();
+//simpl ();
+//simplifier ();
+simpl ();
+  l_to_r [`ifte_lift_prob_wbind];
+
+(*
+ prob_wbind (ifte c (lift_pure_prob_wp (pure_return unit ())) (prob_admit_wp unit))
+                  (fun _ x -> prob_wreturn 0 x)
+              else
+              *)
+              
+dump"test8a";
+admit_all()) =
+  if c then probr 0 else probr 1
+
+
+
+// FAILS
+let test8 () : Prob nat (fun p -> (p 0 +. p 1) /. two) by (
+split();
+smt();
+split();
+split();
+let c = forall_intro() in
+unfold_def(`pure_null_wp);
+smt();
+unfold_def(`pure_null_wp);
+smt();
+
+
+squash_intro();
+dump"before";
+apply_lemma (`strongerI);
+norm[];
+let post = forall_intro() in
+norm [delta_only ["ProbabilismWP.prob_wbind"]];
+l_to_r [`on_beta];
+//l_to_r [`prob_wbind_beta];
+norm [simplify];
+l_to_r [`bool_simp1; `bool_simp2; `bool_simp3; `bool_simp4];
+norm [simplify];
+l_to_r[`largest_single; `simp1; `simp2];
+norm [simplify];
+
+dump"";
+admit_all() ) =
+   let c : bool = coin() in 0 // (if c then 0 else 1)
+
+// FAILS
+// let test9 () : Prob bool (fun post -> (post true +. post false) /. two) =
+//   (if coin () then coin() else coin())
+
+// FAILS
+// let test10 () : PROB nat (fun p -> (p 0 +. p 1) /. two) =
+//   let c : bool = coin() in
+//   (if true then 0 else 1)
+
+
+(* 
+
+Question:
+
+what happens if we try to build the uniform distribution on sequences?
+
+Approach:
+
+let f n : Prob bool = uniform ()
+let g () : Prob (nat => bool) = "f on all points" --- Doesn't work, so probably we don't have a problem.
+
+*)
