Test.fst
@@ -1,0 +1,13 @@
+module Test
+
+open FStar.Tactics
+
+let empty = _:unit{False}
+let g : unit -> bool = fun x -> true
+let h : unit -> bool = fun x -> false
+let gh (x:empty) : Lemma(g x == h x) = ()
+
+let unsound () : Lemma(False) =
+  assert ((fun (x:empty) -> g x) == (fun (x:empty) -> h x)) by (l_to_r [`gh]); // by substituting
+  assert (g == h);  // by eta-reduction
+  assert (g () == h ())
